theories/unary_lr.v
@@ -33,10 +33,10 @@ Section logrel.
 
   Program Definition def_interp_vmem (interp : listVlC -n> D) :
     listVlC -n> dmC -n> iProp Σ :=
-    λne ρ d, (⌜ fv_n d 0 ⌝ ∗ ∃ vmem, ⌜d = dvl vmem⌝ ∧ ▷ interp ρ vmem)%I.
+    λne ρ d, (⌜ nclosed d 0 ⌝ ∗ ∃ vmem, ⌜d = dvl vmem⌝ ∧ ▷ interp ρ vmem)%I.
 
   Program Definition interp_vmem l (interp : listVlC -n> D) : listVlC -n> D :=
-    λne ρ v, (⌜ fv_n_vl v 0 ⌝ ∗ ∃ d, ⌜v @ l ↘ d⌝ ∧ def_interp_vmem interp ρ d)%I.
+    λne ρ v, (⌜ nclosed_vl v 0 ⌝ ∗ ∃ d, ⌜v @ l ↘ d⌝ ∧ def_interp_vmem interp ρ d)%I.
 
   Definition idm_proj_semtype d σ' (φ : listVlC -n> D) : iProp Σ :=
     (∃ γ, ⌜ d = dtysem σ' γ ⌝ ∗ γ ⤇ (λ vs w, φ vs w))%I.
@@ -46,14 +46,14 @@ Section logrel.
   Program Definition def_interp_tmem (interp1 interp2 : listVlC -n> D) :
     listVlC -n> dmC -n> iProp Σ :=
     λne ρ d,
-    (⌜ fv_n d 0 ⌝ ∗ ∃ φ σ, (d ↗ σ , φ) ∗
-       □ ((∀ v, ⌜ fv_n_vl v 0 ⌝ → ▷ interp1 ρ v → ▷ □ φ σ v) ∗
-          (∀ v, ⌜ fv_n_vl v 0 ⌝ → ▷ □ φ σ v → ▷ interp2 ρ v) ∗
+    (⌜ nclosed d 0 ⌝ ∗ ∃ φ σ, (d ↗ σ , φ) ∗
+       □ ((∀ v, ⌜ nclosed_vl v 0 ⌝ → ▷ interp1 ρ v → ▷ □ φ σ v) ∗
+          (∀ v, ⌜ nclosed_vl v 0 ⌝ → ▷ □ φ σ v → ▷ interp2 ρ v) ∗
           (∀ v, interp1 ρ v → interp2 ρ v)))%I.
 
   Program Definition interp_tmem l (interp1 interp2 : listVlC -n> D) : listVlC -n> D :=
     λne ρ v,
-    (⌜ fv_n_vl v 0 ⌝ ∗ ∃ d, ⌜ v @ l ↘ d ⌝ ∧ def_interp_tmem interp1 interp2 ρ d)%I.
+    (⌜ nclosed_vl v 0 ⌝ ∗ ∃ d, ⌜ v @ l ↘ d ⌝ ∧ def_interp_tmem interp1 interp2 ρ d)%I.
 
   Program Definition interp_expr (φ : listVlC -n> D) : listVlC -n> tmC -n> iProp Σ :=
     λne ρ t, WP t {{ φ ρ }} %I.
@@ -65,11 +65,11 @@ Section logrel.
     λne ρ v, (interp1 ρ v ∨ interp2 ρ v) %I.
 
   Program Definition interp_later (interp : listVlC -n> D) : listVlC -n> D :=
-    λne ρ v, (⌜ fv_n_vl v 0 ⌝ ∗ ▷ (interp ρ v)) % I.
+    λne ρ v, (⌜ nclosed_vl v 0 ⌝ ∗ ▷ (interp ρ v)) % I.
 
   Program Definition interp_nat : listVlC -n> D := λne ρ v, (∃ n, ⌜v = vnat n⌝) %I.
 
-  Program Definition interp_top : listVlC -n> D := λne ρ v, ⌜ fv_n_vl v 0 ⌝%I.
+  Program Definition interp_top : listVlC -n> D := λne ρ v, ⌜ nclosed_vl v 0 ⌝%I.
 
   Program Definition interp_bot : listVlC -n> D := λne ρ v, False%I.
 
@@ -87,7 +87,7 @@ Section logrel.
    *)
   Program Definition interp_forall (interp1 interp2 : listVlC -n> D) : listVlC -n> D :=
     λne ρ v,
-    (⌜ fv_n_vl v 0 ⌝ ∗ □ ∀ w, interp1 ρ w -∗ interp_expr interp2 (w :: ρ) (tapp (tv v) (tv w)))%I.
+    (⌜ nclosed_vl v 0 ⌝ ∗ □ ∀ w, interp1 ρ w -∗ interp_expr interp2 (w :: ρ) (tapp (tv v) (tv w)))%I.
 
   Program Definition interp_mu (interp : listVlC -n> D) : listVlC -n> D :=
     λne ρ v, interp (v::ρ) v.
@@ -160,7 +160,7 @@ Section logrel.
 
   Require Import Dot.synLemmas.
 
-  Lemma interp_v_closed T v ρ: (interp T ρ v → ⌜ fv_n_vl v 0 ⌝)%I.
+  Lemma interp_v_closed T v ρ: (interp T ρ v → ⌜ nclosed_vl v 0 ⌝)%I.
   Proof.
     iInduction T as [] "IHT" forall (ρ v); iIntros "#HT //="; try by iDestruct "HT" as "[% _]".
     (* move: ρ v; induction T; iIntros (ρ v) "HT //="; try solve [by iDestruct "HT" as "[% _]"]. *)
@@ -171,7 +171,7 @@ Section logrel.
     - iDestruct "HT" as (n) "%"; subst. iPureIntro. solve_fv_congruence.
   Qed.
 
-  Lemma def_interp_v_closed T d l ρ: (def_interp T l ρ d → ⌜ fv_n d 0 ⌝)%I.
+  Lemma def_interp_v_closed T d l ρ: (def_interp T l ρ d → ⌜ nclosed d 0 ⌝)%I.
   Proof.
     iInduction T as [] "IH" forall (ρ d); iIntros "#HT //="; by iDestruct "HT" as "[% [% _]]".
   Qed.
@@ -189,7 +189,7 @@ Section logrel.
   Program Fixpoint defs_interp (T: ty) : listVlC -n> dmsC -n> iProp Σ :=
     match T with
     | TAnd T1 T2 => defs_interp_and (defs_interp T1) (def_interp T2)
-    | TTop => λne ρ ds, ⌜ fv_n ds 0 ⌝
+    | TTop => λne ρ ds, ⌜ nclosed ds 0 ⌝
     | _ => λne ρ ds, False
     end % I.
 
@@ -199,7 +199,7 @@ Section logrel.
     revert ds ρ; induction T; simpl; intros; try case_match; try apply _.
   Qed.
 
-  Lemma defs_interp_v_closed T ds ρ: (defs_interp T ρ ds → ⌜ fv_n ds 0 ⌝)%I.
+  Lemma defs_interp_v_closed T ds ρ: (defs_interp T ρ ds → ⌜ nclosed ds 0 ⌝)%I.
   Proof.
     iInduction T as [] "IH" forall (ρ ds); iIntros "#HT //=".
     destruct ds. done.
@@ -232,40 +232,40 @@ Section logrel.
   (** Definitions for semantic (definition) (sub)typing *)
   (** Since [⟦Γ⟧* ρ] might be impossible, we must require closedness explicitly. *)
   Definition idtp Γ T l d : iProp Σ :=
-    (⌜ fv_n d (length Γ) ⌝ ∗ □∀ ρ, ⟦Γ⟧* ρ → def_interp T l ρ d.|[to_subst ρ])%I.
+    (⌜ nclosed d (length Γ) ⌝ ∗ □∀ ρ, ⟦Γ⟧* ρ → def_interp T l ρ d.|[to_subst ρ])%I.
   Global Arguments idtp /.
   Notation "Γ ⊨d { l = d } : T" := (idtp Γ T l d) (at level 64, l, d, T at next level).
 
-  Lemma idtp_closed Γ T l d: (Γ ⊨d {l = d} : T → ⌜ fv_n d (length Γ) ⌝)%I.
+  Lemma idtp_closed Γ T l d: (Γ ⊨d {l = d} : T → ⌜ nclosed d (length Γ) ⌝)%I.
   Proof. iIntros "[$ _]". Qed.
 
   Definition idstp Γ T ds : iProp Σ :=
-    (⌜ fv_n ds (length Γ) ⌝ ∗ □∀ ρ, ⟦Γ⟧* ρ → defs_interp T ρ ds.|[to_subst ρ])%I.
+    (⌜ nclosed ds (length Γ) ⌝ ∗ □∀ ρ, ⟦Γ⟧* ρ → defs_interp T ρ ds.|[to_subst ρ])%I.
   Global Arguments idstp /.
   Notation "Γ ⊨ds ds : T" := (idstp Γ T ds) (at level 74, ds, T at next level).
 
-  Lemma idstp_closed Γ T ds: (Γ ⊨ds ds : T → ⌜ fv_n ds (length Γ) ⌝)%I.
+  Lemma idstp_closed Γ T ds: (Γ ⊨ds ds : T → ⌜ nclosed ds (length Γ) ⌝)%I.
   Proof. iIntros "[$ _]". Qed.
 
   Notation "⟦ T ⟧ₑ" := (interp_expr (interp T)).
 
   (* Really needed? Try to stop using it. *)
-  Definition ivtp Γ T v : iProp Σ := (⌜ fv_n_vl v (length Γ) ⌝ ∗ □∀ ρ, ⟦Γ⟧* ρ → ⟦T⟧ ρ v.[to_subst ρ])%I.
+  Definition ivtp Γ T v : iProp Σ := (⌜ nclosed_vl v (length Γ) ⌝ ∗ □∀ ρ, ⟦Γ⟧* ρ → ⟦T⟧ ρ v.[to_subst ρ])%I.
   Global Arguments ivtp /.
 
-  Definition ietp Γ T e : iProp Σ := (⌜ fv_n e (length Γ) ⌝ ∗ □∀ ρ, ⟦Γ⟧* ρ → ⟦T⟧ₑ ρ (e.|[to_subst ρ]))%I.
+  Definition ietp Γ T e : iProp Σ := (⌜ nclosed e (length Γ) ⌝ ∗ □∀ ρ, ⟦Γ⟧* ρ → ⟦T⟧ₑ ρ (e.|[to_subst ρ]))%I.
   Global Arguments ietp /.
   Notation "Γ ⊨ e : T" := (ietp Γ T e) (at level 74, e, T at next level).
 
-  Lemma ietp_closed Γ T e: (Γ ⊨ e : T → ⌜ fv_n e (length Γ) ⌝)%I.
+  Lemma ietp_closed Γ T e: (Γ ⊨ e : T → ⌜ nclosed e (length Γ) ⌝)%I.
   Proof. iIntros "[$ _]". Qed.
 
   Definition step_indexed_ietp Γ T e i: iProp Σ :=
-    (⌜ fv_n e (length Γ) ⌝ ∗ □∀ ρ, ⟦Γ⟧* ρ → ▷^i ⟦T⟧ₑ ρ (e.|[to_subst ρ]))%I.
+    (⌜ nclosed e (length Γ) ⌝ ∗ □∀ ρ, ⟦Γ⟧* ρ → ▷^i ⟦T⟧ₑ ρ (e.|[to_subst ρ]))%I.
   Global Arguments step_indexed_ietp /.
   Notation "Γ ⊨ e : T , i" := (step_indexed_ietp Γ T e i) (at level 74, e, T at next level).
 
-  Lemma step_indexed_ietp_closed Γ T e i: (Γ ⊨ e : T, i → ⌜ fv_n e (length Γ) ⌝)%I.
+  Lemma step_indexed_ietp_closed Γ T e i: (Γ ⊨ e : T, i → ⌜ nclosed e (length Γ) ⌝)%I.
   Proof. iIntros "[$ _]". Qed.
 
   (** Subtyping. Defined on values. *)
@@ -275,7 +275,7 @@ Section logrel.
   (** Indexed Subtyping. Defined on closed values. We must require closedness
       explicitly, since closedness now does not follow from being well-typed later. *)
   Definition step_indexed_ivstp Γ T1 T2 i j: iProp Σ :=
-    (□∀ ρ v, ⌜ fv_n_vl v 0 ⌝ → ⟦Γ⟧*ρ → (▷^i ⟦T1⟧ ρ v) → ▷^j ⟦T2⟧ ρ v)%I.
+    (□∀ ρ v, ⌜ nclosed_vl v 0 ⌝ → ⟦Γ⟧*ρ → (▷^i ⟦T1⟧ ρ v) → ▷^j ⟦T2⟧ ρ v)%I.
   Global Arguments step_indexed_ivstp /.
 
   Global Instance idtp_persistent Γ T l d: Persistent (idtp Γ T l d) := _.
@@ -308,7 +308,7 @@ Section logrel_lemmas.
   Context `{HdotG: dotG Σ}.
 
   Lemma iterate_TLater_later i T ρ v:
-    fv_n_vl v 0 →
+    nclosed_vl v 0 →
     ⟦ iterate TLater i T ⟧ ρ v ≡ (▷^i ⟦ T ⟧ ρ v)%I.
   Proof.
     elim: i => [|i IHi] // => Hcl. rewrite iterate_S /= IHi //.
@@ -381,13 +381,13 @@ Section logrel_lemmas.
     cl_ρ ρ → ⟦ τ.|[to_subst ρ] ⟧ [] v ≡ ⟦ τ ⟧ ρ v.
   Proof.
     elim: ρ τ => /= [|w ρ IHρ] τ Hwρcl; asimpl; first by [].
-    assert (fv_n_vl w 0 /\ Forall (λ v, fv_n_vl v 0) ρ) as [Hwcl Hρcl]. by inversion Hwρcl.
+    assert (nclosed_vl w 0 /\ Forall (λ v, nclosed_vl v 0) ρ) as [Hwcl Hρcl]. by inversion Hwρcl.
     specialize (IHρ (τ.|[w/]) Hρcl).
     asimpl in IHρ. move: IHρ. rewrite closed_subst_vl_id// => IHρ.
     rewrite IHρ -interp_subst closed_subst_vl_id //.
   Qed.
 
-  Lemma to_subst_interp T ρ v w: cl_ρ ρ → fv_n_vl v (length ρ) →
+  Lemma to_subst_interp T ρ v w: cl_ρ ρ → nclosed_vl v (length ρ) →
     ⟦ T.|[v/] ⟧ ρ w ≡ ⟦ T.|[v.[to_subst ρ]/] ⟧ ρ w.
   Proof.
     intros Hclρ Hclv.
@@ -410,19 +410,19 @@ Section logrel_lemmas.
     iPureIntro; by constructor.
   Qed.
 
-  Lemma interp_env_to_subst_closed ρ x: x < length ρ → (⟦ Γ ⟧* ρ → ⌜ fv_n_vl (to_subst ρ x) 0 ⌝)%I.
+  Lemma interp_env_to_subst_closed ρ x: x < length ρ → (⟦ Γ ⟧* ρ → ⌜ nclosed_vl (to_subst ρ x) 0 ⌝)%I.
   Proof.
     iIntros (Hl) "#HG". iPoseProof (interp_env_ρ_closed with "HG") as "%".
     iPureIntro; by apply closed_to_subst.
   Qed.
 
-  Lemma ietp_closed_vl T v: (Γ ⊨ tv v : T → ⌜ fv_n_vl v (length Γ) ⌝)%I.
+  Lemma ietp_closed_vl T v: (Γ ⊨ tv v : T → ⌜ nclosed_vl v (length Γ) ⌝)%I.
   Proof.
     iIntros "H".
     iPoseProof (ietp_closed with "H") as "%". by iPureIntro; apply fv_tv_inv.
   Qed.
 
-  (* Lemma interp_env_to_subst_closed ρ x: x < length ρ → (⟦ Γ ⟧* ρ → ⌜ fv_n_vl (to_subst ρ x) 0 ⌝)%I. *)
+  (* Lemma interp_env_to_subst_closed ρ x: x < length ρ → (⟦ Γ ⟧* ρ → ⌜ nclosed_vl (to_subst ρ x) 0 ⌝)%I. *)
   (* Proof. *)
   (*   (* Hint Resolve defs_interp_v_closed def_interp_v_closed interp_v_closed. *) *)
   (*   revert Γ ρ x. *)
@@ -432,7 +432,7 @@ Section logrel_lemmas.
   (* Qed. *)
 
   (* Lemma interp_subst_closed T v w ρ: *)
-  (*   fv_n_vl v (length ρ) → *)
+  (*   nclosed_vl v (length ρ) → *)
   (*   (⟦ Γ ⟧* ρ → ⟦ T.|[v/] ⟧ ρ w ∗-∗ ⟦ T ⟧ (v.[to_subst ρ] :: ρ) w)%I. *)
   (* Proof. *)
   (*   iIntros (Hcl) "#HG". *)
@@ -452,7 +452,7 @@ Section logrel_lemmas.
 
   (* Try giving a simpler proof: *)
   Lemma interp_subst_closed_aux T v w ρ:
-    fv_n_vl v (length ρ) →
+    nclosed_vl v (length ρ) →
     (⟦ Γ ⟧* ρ → ⟦ T.|[v/] ⟧ ρ w ∗-∗ ⟦ T ⟧ (v.[to_subst ρ] :: ρ) w)%I.
   Proof.
     iIntros (Hcl) "#Hg".
@@ -463,7 +463,7 @@ Section logrel_lemmas.
   Qed.
 
   Lemma interp_subst_closed T v w ρ:
-    fv_n_vl v (length Γ) →
+    nclosed_vl v (length Γ) →
     (⟦ Γ ⟧* ρ → ⟦ T.|[v/] ⟧ ρ w ∗-∗ ⟦ T ⟧ (v.[to_subst ρ] :: ρ) w)%I.
   Proof.
     iIntros (Hcl) "#Hg".
